Simplification in closure conversion spec that results in a simpler and ore efficient closure conversion and a simpler proof

theories/L6_PCPS/Heap/closure_conversion.v
@@ -38,67 +38,71 @@ Section CC.
 
   Inductive project_var :
     Ensemble var -> (* Variables in the current scope *)
+    Ensemble var -> (* Functions not yet constructed *)
     cTag -> (* tag of the current environment constructor *)
     var -> (* The environment argument *)
     list var -> (* The environment *)
-    Ensemble var -> (* The free set *)
     var -> (* Before projection *)
-    var -> (* After projection *)
     exp_ctx -> (* Context that will perform the projection *)
-    Ensemble var -> (* The new free set *)
+    Ensemble var -> (* New current scope *)
     Prop :=
   | Var_in_Scope :
-      forall Scope c Γ FVs S x,
+      forall Scope Funs c Γ FVs x,
         x \in Scope ->
-        project_var Scope c Γ FVs S x x Hole_c S
+        project_var Scope Funs c Γ FVs x Hole_c Scope
+  | Var_in_Funs :
+      forall Scope Funs c Γ FVs f,
+        ~ f \in Scope ->
+        f \in Funs ->                      
+        (* adds the function in scope so that it's not constructed again *)
+        project_var Scope Funs c Γ FVs f
+                    (Econstr_c f clo_tag [f ; Γ] Hole_c) (f |: Scope)
   | Var_in_FVs :
-      forall Scope c Γ FVs S x y N,
+      forall Scope Funs c Γ FVs x N,
         ~ x \in Scope ->
+        ~ x \in Funs ->
         nthN FVs N = Some x ->
-        y \in S ->
-        project_var Scope c Γ FVs S x y
-                    (Eproj_c y c N Γ Hole_c) (S \\ [set y]).
+        (* adds the var in scope so that it's not projected again *)
+        project_var Scope Funs c Γ FVs x
+                    (Eproj_c x c N Γ Hole_c) (x |: Scope).
   
   Inductive project_vars :
     Ensemble var -> (* Variables in the current scope *)
+    Ensemble var -> (* Functions not yet constructed *)
     cTag -> (* tag of the current environment constructor *)
     var -> (* The environment argument *)
     list var -> (* The free variables *)
-    Ensemble var -> (* The free set *)
     list var -> (* Before projection *)
-    list var -> (* After projection *)
     exp_ctx -> (* Context that will perform the projection *)
-    Ensemble var -> (* The new free set *)
+    Ensemble var -> (* New current scope *)
     Prop :=
   | VarsNil :
-      forall Scope c Γ FVs S,
-        project_vars Scope c Γ FVs S [] [] Hole_c S
+      forall Scope Funs c Γ FVs,
+        project_vars Scope Funs c Γ FVs [] Hole_c Scope
   | VarsCons :
-      forall Scope c Γ FVs y y' ys ys' C1 C2 S1 S2 S3,
-        project_var Scope c Γ FVs S1 y y' C1 S2 ->
-        project_vars Scope c Γ FVs S2 ys ys' C2 S3 ->
-        project_vars Scope c Γ FVs S1 (y :: ys) (y' :: ys') (comp_ctx_f C1 C2) S3.
+      forall Scope1 Scope2 Scope3 Funs c Γ FVs y ys C1 C2,
+        project_var Scope1 Funs c Γ FVs y C1 Scope2 ->
+        project_vars Scope2 Funs c Γ FVs ys C2 Scope3 ->
+        project_vars Scope1 Funs c Γ FVs (y :: ys) (comp_ctx_f C1 C2) Scope3.
 
-  Inductive make_closures :
-    fundefs -> (* The function block *)
-    var -> (* The environment variable *)
-    exp_ctx -> (* The context that constructs the closures *)
-    Prop :=
-  | closures_Fnil :
-      forall Γ,
-        make_closures Fnil Γ Hole_c
-  | closures_Fcons :
-      forall f xs t e B Γ C,
-        make_closures B Γ C ->
-        make_closures (Fcons f t xs e B) Γ
-                      (Econstr_c f clo_tag [f ; Γ] C).
-
-  (* TODO delete after comp *)
-  Notation "a &: B" := (Intersection _ [set a] B) (at level 48, left associativity)
-                     : Ensembles_scope.
+  (* Not needed anymore *)
+  (* Inductive make_closures : *)
+  (*   fundefs -> (* The function block *) *)
+  (*   var -> (* The environment variable *) *)
+  (*   exp_ctx -> (* The context that constructs the closures *) *)
+  (*   Prop := *)
+  (* | closures_Fnil : *)
+  (*     forall Γ, *)
+  (*       make_closures Fnil Γ Hole_c *)
+  (* | closures_Fcons : *)
+  (*     forall f xs t e B Γ C, *)
+  (*       make_closures B Γ C -> *)
+  (*       make_closures (Fcons f t xs e B) Γ *)
+  (*                     (Econstr_c f clo_tag [f ; Γ] C). *)
   
   Inductive Closure_conversion :
     Ensemble var -> (* Variables in the current scope *)
+    Ensemble var -> (* Functions that are not yet constructed *)
     cTag -> (* tag of the current environment constructor *)
     var -> (* The environment argument *)
     list var -> (* The free variables - need to be ordered *)
@@ -107,77 +111,63 @@ Section CC.
     exp_ctx -> (* The context that the output expression should be put in *)
     Prop :=
   | CC_Econstr :
-      forall Scope c Γ FVs S' S x ys ys' C C' t e e',
-        (* Variables for projected vars should not shadow the variables in
-         scope, i.e. Scope U σ[Funs] U { Γ } *)
-        Disjoint _ S (FV_cc Scope Γ) ->
-        project_vars Scope c Γ FVs S ys ys' C S' ->
-        (* We do not care about ys'. Should never be accessed again so do not
-         add them aτ the current scope *)
-        Closure_conversion (x |: Scope) c Γ FVs e e' C' ->
-        Closure_conversion Scope c Γ FVs (Econstr x t ys e)
-                           (Econstr x t ys' (C' |[ e' ]|)) C
+      forall Scope Scope' Funs c Γ FVs x ys C C' t e e',
+        project_vars Scope Funs c Γ FVs ys C Scope' ->
+        Closure_conversion (x |: Scope') Funs c Γ FVs e e' C' ->
+        Closure_conversion Scope Funs c Γ FVs (Econstr x t ys e)
+                           (Econstr x t ys (C' |[ e' ]|)) C
   | CC_Ecase :
-      forall Scope c Γ FVs x x' C S S' pats pats',
-        Disjoint _ S (FV_cc Scope Γ) ->
-        project_var Scope c Γ FVs S x x' C S' ->
+      forall Scope Scope' Funs c Γ FVs x C pats pats',
+        project_var Scope Funs c Γ FVs x C Scope' ->
         Forall2 (fun (pat pat' : cTag * exp) =>
                    (fst pat) = (fst pat') /\
                    exists C' e',
                      snd pat' = C' |[ e' ]| /\
-                     Closure_conversion Scope c Γ FVs (snd pat) e' C')
+                     Closure_conversion Scope' Funs c Γ FVs (snd pat) e' C')
                 pats pats' ->
-        Closure_conversion Scope c Γ FVs (Ecase x pats) (Ecase x' pats') C
+        Closure_conversion Scope Funs c Γ FVs (Ecase x pats) (Ecase x pats') C
   | CC_Eproj :
-      forall Scope c Γ FVs S S' x y y' C C' t N e e',
-        Disjoint _ S (FV_cc Scope Γ) ->
-        project_var Scope c Γ FVs S y y' C S' ->
-        Closure_conversion (x |: Scope) c Γ FVs e e' C' ->
-        Closure_conversion Scope c Γ FVs (Eproj x t N y e)
-                           (Eproj x t N y' (C' |[ e' ]|)) C
+      forall Scope Scope' Funs c Γ FVs x y C C' t N e e',
+        project_var Scope Funs c Γ FVs y C Scope' ->
+        Closure_conversion (x |: Scope') Funs c Γ FVs e e' C' ->
+        Closure_conversion Scope Funs c Γ FVs (Eproj x t N y e)
+                           (Eproj x t N y (C' |[ e' ]|)) C
   | CC_Efun :
-      forall Scope c Γ c' Γ' FVs FVs' FVs'' B B' e e' C C' Ce S1 S1',
+      forall Scope Scope' Funs c Γ c' Γ' FVs FVs' B B' e e' C Ce,
         (* The environment contains all the variables that are free in B *)
         (occurs_free_fundefs B) <--> (FromList FVs') ->
         (* needed for cost preservation *)
         NoDup FVs' ->
-        (* Project the FVs to construct the environment *)
-        Disjoint _ S1 (FV_cc Scope Γ) ->
-        project_vars Scope c Γ FVs S1 FVs' FVs'' C' S1' ->
+        project_vars Scope Funs c Γ FVs FVs' C Scope' ->
         (* Γ' is the variable that will hold the record of the environment *)
         ~ Γ' \in ((name_in_fundefs B) :|: (FV_cc Scope Γ)) ->
-        make_closures B Γ' C ->
         (* closure convert function blocks *)
         Closure_conversion_fundefs B c' FVs' B B' ->
         (* closure convert the rest of the program *)
-        Closure_conversion (name_in_fundefs B :|: Scope) c Γ FVs e e' Ce  ->
-        Closure_conversion Scope c Γ FVs (Efun B e)
-                           (Efun B' (C |[ Ce |[ e' ]| ]|)) (comp_ctx_f C' (Econstr_c Γ' c' FVs'' Hole_c))
+        Closure_conversion Scope' (name_in_fundefs B :|: Funs) c Γ FVs e e' Ce  ->
+        Closure_conversion Scope Funs c Γ FVs (Efun B e)
+                           (Efun B' (Ce |[ e' ]|)) (comp_ctx_f C (Econstr_c Γ' c' FVs' Hole_c))
   | CC_Eapp :
-      forall Scope c Γ FVs f f' f'' ft env' ys ys' C S S',
+      forall Scope Scope' Funs c Γ FVs f f' ft env' ys C S S',
         Disjoint _ S (FV_cc Scope Γ) ->
         (* Project the function name and the actual parameter *)
-        project_vars Scope c Γ FVs S (f :: ys) (f' :: ys') C S' ->
-        (* (* Project the actual parameters *) *)
-        (* project_vars Scope Γ FVs S1 ys ys' C2 S2 -> *)
+        project_vars Scope Funs c Γ FVs (f :: ys) C Scope' ->
         (* The name of the function pointer and the name of the environment
          should not shadow the variables in the current scope and the
          variables that where used in the projections *)
-        f'' \in S' -> env' \in S' -> f'' <> env' ->
-        Closure_conversion Scope c Γ FVs (Eapp f ft ys) (AppClo f' ft ys' f'' env') C
+        f' \in S' -> env' \in S' -> f' <> env' ->
+        Closure_conversion Scope Funs c Γ FVs (Eapp f ft ys) (AppClo f ft ys f' env') C
   | CC_Eprim :
-      forall Scope c Γ FVs S S' x ys ys' C C' f e e',
-        Disjoint _ S (FV_cc Scope Γ) ->
-        project_vars Scope c Γ FVs S ys ys' C S' ->
-        Closure_conversion (x |: Scope) c Γ FVs e e' C' ->
-        Closure_conversion Scope c Γ FVs (Eprim x f ys e)
-                           (Eprim x f ys' (C' |[ e' ]|)) C
+      forall Scope Scope' Funs c Γ FVs x ys C C' f e e',
+        project_vars Scope Funs c Γ FVs ys C Scope' ->
+        Closure_conversion (x |: Scope') Funs c Γ FVs e e' C' ->
+        Closure_conversion Scope Funs c Γ FVs (Eprim x f ys e)
+                           (Eprim x f ys (C' |[ e' ]|)) C
   | CC_Ehalt :
-      forall Scope c Γ FVs x x' C S S',
-        Disjoint _ S (FV_cc Scope Γ) ->
+      forall Scope Scope' Funs c Γ FVs x C,
         (* Project the function name and the actual parameter *)
-        project_var Scope c Γ FVs S x x' C S' ->
-        Closure_conversion Scope c Γ FVs (Ehalt x) (Ehalt x') C
+        project_var Scope Funs c Γ FVs x C Scope' ->
+        Closure_conversion Scope Funs c Γ FVs (Ehalt x) (Ehalt x) C
   with Closure_conversion_fundefs :
          fundefs -> (* The current block. Needed to make closures upon entry. *)
          cTag -> (* tag of the current environment constructor *)
@@ -186,18 +176,16 @@ Section CC.
          fundefs -> (* After cc *)
          Prop :=
        | CC_Fccons :
-           forall B c Γ' FVs S f t ys e e' Cf C defs defs',
+           forall B c Γ' FVs S f t ys e e' C defs defs',
              (* The environment binding should not shadow the current scope
                (i.e. the names of the mut. rec. functions and the other arguments) *)
              Disjoint _ S ((name_in_fundefs B) :|: (FromList ys) :|: (bound_var e)) ->
              (* new argument *)
              In _ S  Γ' ->
-             make_closures B  Γ' Cf -> 
              Closure_conversion_fundefs B c FVs defs defs' ->
-             Closure_conversion (FromList ys :|: name_in_fundefs B)
-                                c Γ' FVs e e' C ->
+             Closure_conversion (FromList ys) (name_in_fundefs B) c Γ' FVs e e' C ->
              Closure_conversion_fundefs B c FVs (Fcons f t ys e defs )
-                                        (Fcons f t (Γ' :: ys) (Cf |[ (C |[ e' ]|) ]|) defs')
+                                        (Fcons f t (Γ' :: ys) (C |[ e' ]|) defs')
        | CC_Fnil :
            forall B c FVs,
              Closure_conversion_fundefs B c FVs Fnil Fnil.
